Typing.v
@@ -115,14 +115,16 @@ Proof.
       eauto using valid_env_typ_subst, valid_instance_typ_subst,
                   sch_subst_instance, binds_typ_typ_subst
             with kinding_regular.
-  - apply typing_abs with (L := L \u \{X} \u dom E0 \u dom F);    
-      fold (knd_subst X S knd_type);
+  - apply typing_abs with (L := L \u \{X} \u dom E0 \u dom F).
+    + replace knd_type with (knd_subst X S knd_type) by reflexivity.
       eauto using kinding_typ_subst.
-    introv Hn.
-    rewrite <- sch_subst_empty.
-    rewrite <- concat_assoc.
-    rewrite <- env_subst_typ.
-    auto using concat_assoc.
+    + fold (typ_subst X S T1).
+      replace (sch_empty (typ_subst X S T1))
+        with (sch_subst X S (sch_empty T1)) by reflexivity.
+      introv Hn.
+      rewrite <- concat_assoc.
+      rewrite <- env_subst_typ.
+      auto using concat_assoc.
   - apply typing_let
       with (L := L \u \{X} \u dom E0 \u dom F) (M := sch_subst X S M).
     + introv Hf.
@@ -142,5 +144,212 @@ Proof.
       rewrite <- env_subst_typ.
       auto using concat_assoc.
   - apply typing_constructor
-      with (T2 := typ_subst X S T2) (T3 := typ_subst X S T3).
-    + fold (knd_subst X S (knd_range (typ_top CSet.universe) T2)).
+      with (T2 := typ_subst X S T2) (T3 := typ_subst X S T3); auto.
+    + replace (knd_range (typ_top CSet.universe) (typ_subst X S T2))
+        with (knd_subst X S (knd_range (typ_top CSet.universe) T2))
+        by reflexivity.
+      eauto using kinding_typ_subst.
+    + replace
+        (typ_proj CSet.universe (typ_subst X S T2) (CSet.singleton c))
+        with (typ_subst X S
+                (typ_proj CSet.universe T2 (CSet.singleton c)))
+        by reflexivity.
+      replace (typ_constructor c (typ_subst X S T3))
+        with (typ_subst X S (typ_constructor c T3)) by reflexivity.
+      eauto using subtype_typ_subst.
+  - apply typing_match
+      with (T1 := typ_subst X S T1) (T2 := typ_subst X S T2)
+           (T3 := typ_subst X S T3) (T4 := typ_subst X S T4)
+           (T5 := typ_subst X S T5) (T6 := typ_subst X S T6)
+           (T7 := typ_subst X S T7) (L := L); auto.
+    + replace (knd_range (typ_subst X S T2) (typ_bot CSet.universe))
+        with (knd_subst X S (knd_range T2 (typ_bot CSet.universe)))
+        by reflexivity.
+      eauto using kinding_typ_subst.
+    + replace (knd_range (typ_top CSet.universe) (typ_subst X S T4))
+        with (knd_subst X S (knd_range (typ_top CSet.universe) T4))
+        by reflexivity.
+      eauto using kinding_typ_subst.
+    + replace (knd_range (typ_top CSet.universe) (typ_subst X S T6))
+        with (knd_subst X S (knd_range (typ_top CSet.universe) T6))
+        by reflexivity.
+      eauto using kinding_typ_subst.
+    + replace
+        (typ_proj CSet.universe (typ_subst X S T2) (CSet.singleton c))
+        with (typ_subst X S
+                (typ_proj CSet.universe T2 (CSet.singleton c)))
+        by reflexivity.
+      replace (typ_constructor c (typ_subst X S T7))
+        with (typ_subst X S (typ_constructor c T7)) by reflexivity.
+      eauto using subtype_typ_subst.
+    + replace
+        (typ_proj CSet.universe (typ_subst X S T2) (CSet.singleton c))
+        with (typ_subst X S
+                (typ_proj CSet.universe T2 (CSet.singleton c)))
+        by reflexivity.
+      replace
+        (typ_proj CSet.universe (typ_subst X S T4) (CSet.singleton c))
+        with (typ_subst X S
+                (typ_proj CSet.universe T4 (CSet.singleton c)))
+        by reflexivity.
+      eauto using subtype_typ_subst.
+    + replace
+        (typ_proj
+           CSet.universe (typ_subst X S T2) (CSet.cosingleton c))
+        with (typ_subst X S
+                (typ_proj CSet.universe T2 (CSet.cosingleton c)))
+        by reflexivity.
+      replace
+        (typ_proj
+           CSet.universe (typ_subst X S T6) (CSet.cosingleton c))
+        with (typ_subst X S
+                (typ_proj CSet.universe T6 (CSet.cosingleton c)))
+        by reflexivity.
+      eauto using subtype_typ_subst.
+    + replace (sch_empty (typ_variant (typ_subst X S T3)))
+        with (sch_subst X S (sch_empty (typ_variant T3)))
+        by reflexivity.
+      introv Hn.
+      rewrite <- concat_assoc.
+      rewrite <- env_subst_typ.
+      auto using concat_assoc.
+    + replace (sch_empty (typ_variant (typ_subst X S T5)))
+        with (sch_subst X S (sch_empty (typ_variant T5)))
+        by reflexivity.
+      introv Hn.
+      rewrite <- concat_assoc.
+      rewrite <- env_subst_typ.
+      auto using concat_assoc.
+  - apply typing_destruct
+      with (T1 := typ_subst X S T1) (T2 := typ_subst X S T2)
+           (T3 := typ_subst X S T3) (L := L); auto.
+    + replace (knd_range (typ_subst X S T2) (typ_bot CSet.universe))
+        with (knd_subst X S (knd_range T2 (typ_bot CSet.universe)))
+        by reflexivity.
+      eauto using kinding_typ_subst.
+    + replace
+        (typ_proj CSet.universe (typ_subst X S T2) (CSet.singleton c))
+        with (typ_subst X S
+                (typ_proj CSet.universe T2 (CSet.singleton c)))
+        by reflexivity.
+      replace (typ_constructor c (typ_subst X S T3))
+        with (typ_subst X S (typ_constructor c T3)) by reflexivity.
+      eauto using subtype_typ_subst.
+    + replace (sch_empty (typ_subst X S T3))
+        with (sch_subst X S (sch_empty T3)) by reflexivity.
+      introv Hn.
+      rewrite <- concat_assoc.
+      rewrite <- env_subst_typ.
+      auto using concat_assoc.
+  - apply typing_absurd with (T1 := typ_subst X S T1); auto.
+    + replace (knd_range
+                 (typ_bot CSet.universe) (typ_bot CSet.universe))
+        with (knd_subst X S
+                (knd_range (typ_bot CSet.universe)
+                           (typ_bot CSet.universe)))
+        by reflexivity.
+      eauto using kinding_typ_subst.
+    + replace knd_type with (knd_subst X S knd_type) by reflexivity.
+      eauto using kinding_typ_subst.
+Qed.
+
+Lemma typing_typ_subst_l : forall E X K S t T,
+    typing (E & X ~:: K) t T ->
+    kinding E S K ->
+    typing E t (typ_subst X S T).
+Proof.
+  introv Ht Hk.
+  rewrite <- concat_empty_r with (E := E).
+  rewrite <- concat_empty_r with (E := E & X ~:: K) in Ht.
+  replace empty with (env_subst X S empty)
+    by (unfold env_subst; apply map_empty).
+  eauto using typing_typ_subst.
+Qed.      
+
+Lemma typing_typ_substs_l : forall E Xs M Us t T,
+    fresh (dom E) (sch_arity M) Xs ->
+    typing (E & Xs ~::* M) t T ->
+    valid_instance E Us M ->
+    typing E t (typ_substs Xs Us T).
+Proof.
+  introv Hf Ht Hv.
+  generalize dependent Us.
+  generalize dependent M.
+  generalize dependent T.
+  induction Xs; introv Hf Ht Hv.
+  - simpl. simpl in Ht. rewrite concat_empty_r in Ht.
+    auto using typing_weakening_l with valid_instance_validated.
+  - assert (types (sch_arity M) Us) as Hts
+      by auto with valid_instance_regular.
+    destruct Hts as [Hl2 Hts].
+    destruct Us; destruct M; try discriminate.
+    simpl.
+    fresh_length Hf as Hl1.
+    inversion Hl2.
+    inversion Hl1.
+    inversion Hf.
+    inversion Hv.
+    inversion Hts.
+    subst.
+    apply IHXs with (M := sch_open M t0);
+      autorewrite with rew_sch_arity; eauto.
+    assert (valid_instance E Us (sch_open M t0))
+      as Hv2 by assumption.
+    apply valid_instance_closed with (X := a) in Hv2; auto.
+    assert (a \notin sch_fv M) by eauto using sch_open_fv_inv.
+    rewrite sch_subst_intro with (X := a) (U := t0); auto.
+    rewrite <- env_subst_bind_knds;
+      autorewrite with rew_sch_arity; auto.
+    apply typing_typ_subst with (K := k); auto.
+    rewrite <- concat_assoc.
+    auto.
+Qed.
+
+Lemma typing_instance : forall L E M t Us,
+  (forall Xs,
+    fresh L (sch_arity M) Xs ->
+    typing (E & Xs ~::* M) t (instance_vars M Xs)) ->
+  valid_instance E Us M ->
+  typing E t (instance M Us). 
+Proof.
+  introv Hs Hv.
+  pick_freshes (sch_arity M) Xs.
+  rewrite typ_substs_intro_instance with (Xs := Xs);
+    auto with valid_instance_regular.
+  apply typing_typ_substs_l with (M := M); auto.
+Qed.
+
+Lemma typing_trm_subst : forall L E F x M s t T,
+    typing (E & x ~: M & F) t T ->
+    (forall Xs,
+      fresh L (sch_arity M) Xs ->
+      typing (E & Xs ~::* M) s (instance_vars M Xs)) ->
+    typing (E & F) (trm_subst x s t) T.
+Proof.
+  introv Ht Hs.
+  remember (E & x ~: M & F) as ExF.
+  induction Ht; simpl.
+  - case_var.
+    + subst.
+      assert (environment (E & x ~: M & F)) as He
+        by auto with valid_env_regular.
+      apply ok_from_environment in He.
+      assert (bind_typ M0 = bind_typ M) as Heq
+        by eauto using binds_middle_eq_inv.
+      inversion Heq; subst.
+      assert (valid_env (E & F))
+        by eauto using valid_env_typ_bind.
+      apply typing_instance with (L := L \u dom F);
+        eauto using valid_instance_typ_bind.
+      introv Hf.
+      assert (typing (E & Xs ~::* M) s (instance_vars M Xs)) as Ht
+        by auto.
+      assert (valid_env (E & Xs ~::* M))
+        by auto with typing_validated.
+      apply typing_weakening;
+        auto using valid_env_kinds_weakening_l.
+    + subst.
+      apply typing_var with (M := M0) (Us := Us);
+        eauto using valid_env_typ_bind, valid_instance_typ_bind.
+      apply binds_subst with (x2 := x) (v2 := bind_typ M); auto.
+  - 
